***NO_CI*** more cleanup

examples/preorders/Protocol.fst
@@ -8,10 +8,13 @@ open FStar.ST
 
 open MonotonicArray
 
+(***** basic messages interface *****)
+
 (* size of each message fragment sent over the network *)
 assume val fragment_size:nat
 
 type byte
+assume val zero_b:byte
 
 type message  = s:seq byte{length s <= fragment_size}
 type fragment = s:seq byte{length s = fragment_size}
@@ -19,26 +22,31 @@ type fragment = s:seq byte{length s = fragment_size}
 (* random bytes for ideal cipher? *)
 type randomness = nat -> fragment
 
-assume val oplus: fragment -> fragment -> fragment
+(* the xor operation on fragments *)
+assume val xor: fragment -> fragment -> fragment
 
-assume val lemma_oplus (a:fragment) (b:fragment)
-  :Lemma (oplus (oplus a b) b == a)
-   [SMTPat (oplus (oplus a b) b)]
+(* basic lemma about xor *)
+assume val lemma_xor (a:fragment) (b:fragment)
+  :Lemma (xor (xor a b) b == a)
+   [SMTPat (xor (xor a b) b)]
 
-assume val zeroes: n:nat -> (s:seq byte{length s = n})
+val zeroes: n:nat -> (s:seq byte{length s = n})
+let zeroes n = Seq.create n (zero_b)
 
 let pad (m:message) :fragment = append m (zeroes (fragment_size - (length m)))
 
+(* an unpad function that strips off the trailing pad *)
 assume val unpad (s:fragment)
   :(r:(nat * message){length (snd r) = fst r /\ s == pad (snd r)})
 
 assume val lemma_pad_unpad (x:unit) :Lemma (ensures (forall (m:message). snd (unpad (pad m)) == m))
 
+(* a MAC function, returning a tag *)
 assume val mac: cipher:fragment -> i:nat -> seq byte
 
 (* an entry in the message log *)
 noeq type entry (rand:randomness) =
-  | E: i:nat -> msg:message -> cipher:fragment{oplus (pad msg) (rand i) == cipher} -> tag:seq byte{tag == mac cipher i}
+  | E: i:nat -> msg:message -> cipher:fragment{xor (pad msg) (rand i) == cipher} -> tag:seq byte{tag == mac cipher i}
        -> entry rand
 
 (* sequence of messages *)
@@ -48,7 +56,7 @@ let is_prefix_of (#a:Type) (s1:seq a) (s2:seq a) :Type0
   = length s1 <= length s2 /\
     (forall (i:nat). i < length s1 ==> Seq.index s1 i == Seq.index s2 i)
 
-(* entries are only appended to, typing entries_rel directly as `preorder (entries rand)` doesn't work *)
+(* entries are only appended to *)
 let entries_rel (rand:randomness) :relation (entries rand) =
   fun (es1:entries rand) (es2:entries rand) -> es1 `is_prefix_of` es2
 
@@ -84,53 +92,53 @@ let entries_of (c:connection) :(mref (entries (rand_of c)) (entries_rel (rand_of
   | S _ es   -> es
   | R _ es _ -> es
 
-let contains_connection (h:heap) (c:connection) =
+let live_connection (h:heap) (c:connection) =
   match c with
   | S _ es_ref         -> h `contains` es_ref
   | R _ es_ref ctr_ref -> h `contains` es_ref /\ h `contains` ctr_ref
 
-let recall_connection (c:connection) :ST unit (requires (fun h0 -> True)) (ensures (fun h0 _ h1 -> h0 == h1 /\ h0 `contains_connection` c))
+let recall_connection_liveness (c:connection)
+  :ST unit (requires (fun h0 -> True)) (ensures (fun h0 _ h1 -> h0 == h1 /\ h0 `live_connection` c))
   = match c with
     | S _ es_ref         -> ST.recall es_ref
     | R _ es_ref ctr_ref -> ST.recall es_ref; ST.recall ctr_ref
 
 (* seq of plain messages sent so far on this connection *)
-let log (c:connection) (h:heap{h `contains_connection` c}) :Tot (seq message) =
+let log (c:connection) (h:heap{h `live_connection` c}) :Tot (seq message) =
   ArrayUtils.seq_map (fun (E _ m _ _) -> m) (sel_tot h (entries_of c))
 
 let lemma_prefix_entries_implies_prefix_log
-  (c:connection) (h1:heap) (h2:heap{h1 `contains_connection` c /\ h2 `contains_connection` c})
+  (c:connection) (h1:heap) (h2:heap{h1 `live_connection` c /\ h2 `live_connection` c})
   :Lemma (requires (sel h1 (entries_of c) `is_prefix_of` sel h2 (entries_of c)))
 	 (ensures  (log c h1 `is_prefix_of` log c h2))
 	 [SMTPat (log c h1); SMTPat (log c h2)]
   = ArrayUtils.lemma_map_commutes_with_prefix (fun (E _ m _ _) -> m) (sel h1 (entries_of c)) (sel h2 (entries_of c))
 
-(* current counter for the connection, consider adding the valid refinement? *)
-let ctr (c:connection) (h:heap{h `contains_connection` c}) :Tot nat =
+(* current counter for the connection *)
+let ctr (c:connection) (h:heap{h `live_connection` c}) :Tot nat =
   match c with
   | S _ es_ref    -> length (sel_tot h es_ref)
   | R _ _ ctr_ref -> sel_tot h ctr_ref
 
-let recall_counter (c:connection) :ST unit (requires (fun _ -> True)) (ensures (fun h0 _ h1 -> h0 == h1 /\ h0 `contains_connection` c /\ ctr c h0 <= Seq.length (log c h0)))
-  = recall_connection c;
+(* recall_counter, as mentioned in the paper *)
+let recall_counter (c:connection)
+  :ST unit (requires (fun _ -> True)) (ensures (fun h0 _ h1 -> h0 == h1 /\ h0 `live_connection` c /\ ctr c h0 <= Seq.length (log c h0)))
+  = recall_connection_liveness c;
     match c with
     | S _ _              -> ()
     | R _ es_ref ctr_ref -> let n = !ctr_ref in gst_recall (counter_pred n es_ref)
 
-
 (* stable predicate for counter *)
-let connection_pred (c:connection) (h0:heap{h0 `contains_connection` c}) :(p:heap_predicate{stable p}) =
-  fun h -> h `contains_connection` c /\
+let snapshot_pred (c:connection) (h0:heap{h0 `live_connection` c}) :(p:heap_predicate{stable p}) =
+  fun h -> h `live_connection` c /\
         ctr c h0 <= ctr  c h /\ ctr c h0 <= length (log c h) /\ log c h0 `is_prefix_of` log c h
 
 let snap (c:connection) :ST unit (requires (fun _ -> True))
-                                 (ensures  (fun h0 _ h1 -> h0 `contains_connection` c /\ witnessed (connection_pred c h0) /\ h0 == h1))
+                                 (ensures  (fun h0 _ h1 -> h0 `live_connection` c /\ witnessed (snapshot_pred c h0) /\ h0 == h1))
   = let h0 = ST.get () in
-    recall_connection c;
-    (match c with
-     | S _ _              -> ()
-     | R _ es_ref ctr_ref -> gst_recall (counter_pred (sel_tot h0 ctr_ref) es_ref));
-    gst_witness (connection_pred c h0)
+    recall_connection_liveness c;
+    recall_counter c;
+    gst_witness (snapshot_pred c h0)
 
 type iarray (a:Type0) (n:nat) = x:array a n{all_init x}
 
@@ -143,17 +151,17 @@ let connection_footprint (c:connection) :GTot (Set.set nat)
     | R _ es_ref ctr_ref -> Set.union (Set.singleton (addr_of es_ref)) (Set.singleton (addr_of ctr_ref))
 
 let lemma_snoc_log
-  (c:connection{sender c}) (i:nat) (cipher:fragment) (msg:message{oplus (pad msg) ((rand_of c) i) == cipher})
+  (c:connection{sender c}) (i:nat) (cipher:fragment) (msg:message{xor (pad msg) ((rand_of c) i) == cipher})
   (tag:seq byte{tag == mac cipher i})
-  (h0:heap) (h1:heap{h0 `contains_connection` c /\ h1 `contains_connection` c})
+  (h0:heap) (h1:heap{h0 `live_connection` c /\ h1 `live_connection` c})
   :Lemma (requires (sel h1 (entries_of c) == snoc (sel h0 (entries_of c)) (E i msg cipher tag)))
 	 (ensures  (log c h1 == snoc (log c h0) msg))
   = ArrayUtils.lemma_map_commutes_with_snoc (fun (E _ m _ _) -> m) (sel h0 (entries_of c)) (E i msg cipher tag)
 
-(* network send is called once log had been appended to etc. *)
+(* network send, actually sends bytes on the network, once the log has been prepared *)
 assume val network_send
   (c:connection{sender c}) (f:fragment) (tag:seq byte)
-  :ST unit (requires (fun h0 -> h0 `contains_connection` c /\ 
+  :ST unit (requires (fun h0 -> h0 `live_connection` c /\ 
                              (let S _ es_ref = c in
                               let es = sel h0 es_ref in
 			      Seq.length es > 0 /\
@@ -161,19 +169,20 @@ assume val network_send
 			       c == f /\ t == tag))))
            (ensures  (fun h0 _ h1 -> h0 == h1))
 
+(* protocol send operation *)
 #set-options "--z3rlimit 50"
 let send (#n:nat) (buf:iarray byte n) (c:connection{sender c})
   :ST nat (requires (fun h0 -> True))
         (ensures  (fun h0 sent h1 -> modifies (connection_footprint c) h0 h1         /\
-	                          h0 `contains_connection` c /\
-				  h1 `contains_connection` c /\
+	                          h0 `live_connection` c /\
+				  h1 `live_connection` c /\
 	                          sent <= min n fragment_size /\
 				  ctr c h1 = ctr c h0 + 1    /\
 				  (forall (i:nat). i < n ==> Some? (Seq.index (as_seq buf h0) i)) /\
                                   log c h1 == snoc (log c h0) (as_initialized_subseq buf h0 0 sent)))
   = let h0 = ST.get () in
 
-    recall_connection c;
+    recall_connection_liveness c;
     recall_all_init buf;
 
     let S rand es_ref = c in
@@ -184,7 +193,7 @@ let send (#n:nat) (buf:iarray byte n) (c:connection{sender c})
     let sent = min n fragment_size in
     let msg = read_subseq_i_j buf 0 sent in
     let frag = append msg (zeroes (fragment_size - sent)) in
-    let cipher = oplus frag (rand i0) in
+    let cipher = xor frag (rand i0) in
 
     let msgs1 = snoc msgs0 (E i0 msg cipher (mac cipher i0)) in
 
@@ -201,7 +210,7 @@ let ciphers (c:connection) (h:heap) :GTot (seq fragment) =
   ArrayUtils.seq_map (fun (E _ _ cipher _) -> cipher) (sel h (entries_of c))
 
 assume val network_receive (c:connection)
-  :ST (option (fragment * seq byte)) (requires (fun h0 -> h0 `contains_connection` c))
+  :ST (option (fragment * seq byte)) (requires (fun h0 -> h0 `live_connection` c))
                                      (ensures  (fun h0 _ h1 -> h0 == h1))
 
 let modifies_r (#n:nat) (c:connection{receiver c}) (arr:array byte n) (h0 h1:heap) :Type0
@@ -209,7 +218,7 @@ let modifies_r (#n:nat) (c:connection{receiver c}) (arr:array byte n) (h0 h1:hea
                         (array_footprint arr)) h0 h1
 
 assume val verify (c:connection{receiver c}) (cipher:fragment) (tag:seq byte) (i:nat)
-  :ST bool (requires (fun h0 -> h0 `contains_connection` c))
+  :ST bool (requires (fun h0 -> h0 `live_connection` c))
            (ensures  (fun h0 r h1 -> h0 == h1 /\
 	              (r ==>
 	               (let R _ es_ref _ = c in
@@ -224,8 +233,8 @@ let receive (#n:nat{fragment_size <= n}) (buf:array byte n) (c:connection{receiv
                  (ensures  (fun h0 r_opt h1 -> match r_opt with
 					    | None   -> h0 == h1
 					    | Some r ->
-					      h0 `contains_connection` c   /\
-					      h1 `contains_connection` c   /\
+					      h0 `live_connection` c   /\
+					      h1 `live_connection` c   /\
 					      modifies_r c buf h0 h1       /\
 					      disjoint_siblings_remain_same buf h0 h1 /\
 					      r <= fragment_size            /\
@@ -240,7 +249,7 @@ let receive (#n:nat{fragment_size <= n}) (buf:array byte n) (c:connection{receiv
 
     Set.lemma_disjoint_subset (connection_footprint c) (array_footprint buf) (Set.singleton (addr_of ctr_ref));
 
-    recall_connection c;
+    recall_connection_liveness c;
 
     match network_receive c with
     | None               -> None
@@ -249,7 +258,7 @@ let receive (#n:nat{fragment_size <= n}) (buf:array byte n) (c:connection{receiv
 
       if not (verify c cipher tag i0) then None
       else
-        let msg = oplus cipher (rand i0) in
+        let msg = xor cipher (rand i0) in
         let len, m = unpad msg in
 
 	lemma_pad_unpad ();
@@ -274,17 +283,24 @@ let lemma_is_prefix_of_slice
 	 [SMTPat (s1 `is_prefix_of` s2); SMTPat (Seq.slice s1 i j); SMTPat (Seq.slice s2 i j)]
   = ArrayUtils.lemma_is_prefix_of_slice s1 s2 i j
 
+(*****)
+
+(*
+ * assuming a flattening function that flattens a sequence of messages into sequence of bytes
+ * and a couple of associated lemmas
+ *)
 assume val flatten (s:seq message) :Tot (seq byte)
 
 assume val lemma_flatten_snoc (s:seq message) (m:message)
   :Lemma (requires True)
          (ensures  (flatten (snoc s m) == append (flatten s) m))
 
-assume val flatten_empty (u:unit) : Lemma 
-  (flatten Seq.createEmpty == Seq.createEmpty)
-  
+assume val flatten_empty (u:unit) : Lemma (flatten Seq.createEmpty == Seq.createEmpty)
+
+(*****)
+
 let sent_file_pred' (file:seq byte) (c:connection) (from:nat) (to:nat{from <= to}) :heap_predicate
-  = fun h -> h `contains_connection` c /\ 
+  = fun h -> h `live_connection` c /\ 
           (let log   = log c h in
            to <= Seq.length log /\ 
 	   file == flatten (Seq.slice log from to))
@@ -338,7 +354,7 @@ let append_subseq #a #n (f:iarray a n) (pos:nat) (sent:nat{pos + sent <= n}) (h:
       assert (Seq.equal f1 (append f0 sent_frag))
 
 let lemma_sender_connection_ctr_equals_length_log
-  (c:connection{sender c}) (h:heap{h `contains_connection` c})
+  (c:connection{sender c}) (h:heap{h `live_connection` c})
   :Lemma (ctr c h == Seq.length (log c h))
   = ()
 
@@ -352,12 +368,12 @@ val send_aux
       : ST unit 
              (requires (fun h0 ->
                       file `fully_initialized_in` h0 /\
-                      h0 `contains_connection` c /\
+                      h0 `live_connection` c /\
                       from <= ctr c h0 /\
                       sent_file_pred (as_initialized_subseq file h0 0 pos) c from (ctr c h0) h0))
              (ensures  (fun h0 _ h1 -> 
                       modifies (connection_footprint c) h0 h1 /\
-                      h1 `contains_connection` c /\
+                      h1 `live_connection` c /\
                       from <= ctr c h1 /\
                       (forall (k:nat). k < n ==> Some? (Seq.index (as_seq file h0) k)) /\
                       sent_file_pred (as_initialized_seq file h0) c from (ctr c h1) h1))
@@ -379,7 +395,7 @@ let rec send_aux #n file c from pos
           recall_contains file; //strange that this is needed
           assert (from <= ctr c h1);
           assert (file `fully_initialized_in` h1);
-          assert (h1 `contains_connection` c);
+          assert (h1 `live_connection` c);
           let _ : unit = 
             let sent_frag = as_initialized_subseq sub_file h0 0 sent in
             let sent_frag' = as_initialized_subseq file h0 pos (pos + sent) in
@@ -399,8 +415,6 @@ let rec send_aux #n file c from pos
             assert (f0 == flatten (Seq.slice log0 from (ctr c h0)));
             lemma_flatten_snoc (Seq.slice log0 from (ctr c h0)) sent_frag;
             assert (f1 == flatten (Seq.slice log1 from (ctr c h1)));
-            // assert (f0 == flatten (Seq.slice log1 from (ctr c h0)));
-            // assume (f1 == flatten (Seq.slice log1 from (ctr c h1)));
             assert (sent_file_pred f1 c from (ctr c h1) h1) 
          in
          send_aux file c from (pos + sent)
@@ -410,13 +424,13 @@ let send_file (#n:nat) (file:iarray byte n) (c:connection{sender c /\ Set.disjoi
        (requires (fun h -> True))
        (ensures (fun h0 _ h1 ->
                       modifies (connection_footprint c) h0 h1 /\
-                      h1 `contains_connection` c /\
+                      h1 `live_connection` c /\
                       (forall (k:nat). k < n ==> Some? (Seq.index (as_seq file h0) k)) /\
                       sent_file (as_initialized_seq file h0) c))
   = let h0 = ST.get () in
     recall_all_init file;
     recall_contains file;
-    recall_connection c;
+    recall_connection_liveness c;
     let file_bytes0 = iarray_as_seq file in
     let from = ctr c h0 in
     assert (Seq.equal (as_initialized_subseq file h0 0 0) Seq.createEmpty);
@@ -437,7 +451,7 @@ val receive_aux
           (#n:nat)
           (file:array byte n)
           (c:connection{receiver c /\ Set.disjoint (connection_footprint c) (array_footprint file)})
-          (h_init:heap{h_init `contains_connection` c})
+          (h_init:heap{h_init `live_connection` c})
           (from:nat{from = ctr c h_init})
           (pos:nat{fragment_size <= n - pos})
     : ST (option (r:nat{r <= n}))
@@ -445,12 +459,12 @@ val receive_aux
               let file_in = prefix file pos in
               all_init_i_j file_in 0 pos /\
               file_in `fully_initialized_in` h0 /\
-              h0 `contains_connection` c /\
+              h0 `live_connection` c /\
               from <= ctr c h0 /\
               sent_file_pred (as_initialized_seq file_in h0) c from (ctr c h0) h0))
         (ensures (fun h0 ropt h1 ->
                    modifies_r c file h0 h1 /\
-                   h1 `contains_connection` c /\
+                   h1 `live_connection` c /\
                    (match ropt with
                     | None -> True
                     | Some r ->
@@ -539,7 +553,7 @@ val receive_file (#n:nat{fragment_size <= n})
 let receive_file #n file c = 
   let h_init = ST.get () in
   recall_contains file;
-  recall_connection c;
+  recall_connection_liveness c;
   let R _ es ctr_ref = c in
   let from = !ctr_ref in 
   gst_recall (counter_pred from es);
@@ -565,7 +579,7 @@ let tags (c:connection) (h:heap) :GTot (seq (seq byte)) =
 let lemma_partial_length_hiding
   (#n:nat) (#m:nat)
   (c0:connection{sender c0}) (c1:connection{sender c1})
-  (h:heap{h `contains_connection` c0 /\ h `contains_connection` c1})
+  (h:heap{h `live_connection` c0 /\ h `live_connection` c1})
   (file0:iarray byte n) (file1:iarray byte m)
   (from:nat) (to:nat{from <= to /\ to <= Seq.length (log c0 h) /\ to <= Seq.length (log c1 h)})
   :Lemma (requires (let S rand0 _ = c0 in
@@ -577,8 +591,8 @@ let lemma_partial_length_hiding
 	              sent_file_pred f0 c0 from to h /\
 	              sent_file_pred f1 c1 from to h /\
 	              (forall (i:nat). (i >= from /\ i < to) ==>
-		                 oplus (pad (Seq.index (log c0 h) i)) (rand0 i) ==
-	                         oplus (pad (Seq.index (log c1 h) i)) (rand1 i))))))
+		                 xor (pad (Seq.index (log c0 h) i)) (rand0 i) ==
+	                         xor (pad (Seq.index (log c1 h) i)) (rand1 i))))))
 	 (ensures  (forall (i:nat). (i >= from /\ i < to) ==> (Seq.index (ciphers c0 h) i == Seq.index (ciphers c1 h) i) /\
 	                                              Seq.index (tags c0 h) i == Seq.index (tags c1 h) i))
   = let S rand0 _ = c0 in
@@ -587,7 +601,7 @@ let lemma_partial_length_hiding
     let ciphers1 = ciphers c1 h in
     let tags0 = tags c0 h in
     let tags1 = tags c1 h in
-    assert (forall (i:nat). (i >= from /\ i < to) ==> Seq.index ciphers0 i == oplus (pad (Seq.index (log c0 h) i)) (rand0 i));
-    assert (forall (i:nat). (i >= from /\ i < to) ==> Seq.index ciphers1 i == oplus (pad (Seq.index (log c1 h) i)) (rand1 i));
+    assert (forall (i:nat). (i >= from /\ i < to) ==> Seq.index ciphers0 i == xor (pad (Seq.index (log c0 h) i)) (rand0 i));
+    assert (forall (i:nat). (i >= from /\ i < to) ==> Seq.index ciphers1 i == xor (pad (Seq.index (log c1 h) i)) (rand1 i));
     assert (forall (i:nat). (i >= from /\ i < to) ==> Seq.index tags0 i == mac (Seq.index ciphers0 i) i);
     assert (forall (i:nat). (i >= from /\ i < to) ==> Seq.index tags1 i == mac (Seq.index ciphers1 i) i)
